UniverseAbstractions.lean
@@ -34,3 +34,4 @@ import UniverseAbstractions.Instances.Basic
 import UniverseAbstractions.Instances.FunctorUniverse
 import UniverseAbstractions.Instances.CoFunctorUniverse
 import UniverseAbstractions.Instances.Algebra
+import UniverseAbstractions.Instances.Category
