UniverseAbstractions/Instances/Category.lean
@@ -1,139 +1,57 @@
-#exit
-
 import UniverseAbstractions.Axioms.Universes
 import UniverseAbstractions.Axioms.Universe.Identity
 import UniverseAbstractions.Axioms.Universe.Functors
-import UniverseAbstractions.Axioms.Universe.Singletons
-import UniverseAbstractions.Axioms.Universe.Products
-import UniverseAbstractions.Axioms.Universe.Equivalences
 import UniverseAbstractions.Axioms.CategoryTheory.Basic
-import UniverseAbstractions.Instances.Basic
+import UniverseAbstractions.Axioms.CategoryTheory.Functors
 import UniverseAbstractions.Instances.Utils.Bundled
-
-import UniverseAbstractions.MathlibFragments.CoreExt
 
 
 
 set_option autoBoundImplicitLocal false
 --set_option pp.universes true
-set_option synthInstance.maxHeartbeats 10000
 
-universe u u' v iv
-
+universe u v w iw
 
 
-class Category (V : Universe.{v}) [HasIdentity.{v, iv} V] [HasInternalFunctors V] [HasFullFunOp V]
-               (α : Type (max u v iv)) :
-  Type (max u v iv) where
-(M                  : MetaRelation α V)
-[hCategory          : MetaRelation.IsCategory M]
-[I                  : MetaRelation α V]
-[hGroupoid          : MetaRelation.IsGroupoid I]
-(isoToHom (a b : α) : I a b ⟶ M a b)
--- TODO: isoToHom must be functor of categories
 
-namespace Category
+namespace CategoryTheory.IsCategory
 
-  open MetaRelation HasFunctors HasCongrArg HasLinearFunOp IsAssociative IsCategoricalPreorder Bundled
+  open Bundled MetaRelation HasFunctors HasCongrArg HasLinearFunOp IsAssociative IsCategoricalPreorder
 
-  @[reducible] def typeClass (V : Universe.{v}) [HasIdentity.{v, iv} V] [HasInternalFunctors V] [HasFullFunOp V] :
-    SimpleTypeClass.{(max u v iv) + 1, (max u v iv) + 1} := Category.{u, v, iv} V
-  @[reducible] def univ (V : Universe.{v}) [HasIdentity.{v, iv} V] [HasInternalFunctors V] [HasFullFunOp V] :
-    Universe := Bundled.univ.{u + 1, (max u v iv) + 1} (typeClass.{u, v, iv} V)
+  def typeClass (M : IsoUniverse.{w, iw}) :
+    SimpleTypeClass.{max u (w + 1) iw, max u (w + 1) iw} := IsCategory.{max u (w + 1) iw, w, iw} M
+  def univ (M : IsoUniverse.{w, iw}) :
+    Universe.{max u (w + 1) iw} := Bundled.univ.{max u (w + 1) iw, max u (w + 1) iw} (typeClass.{u} M)
 
-  variable {V : Universe.{v}} [HasIdentity.{v, iv} V] [HasInternalFunctors V] [HasFullFunOp V]
+  variable {M : IsoUniverse.{w, iw}}
 
-  instance inst (A : univ.{u, v, iv} V) : Category.{u, v, iv} V ⌈A⌉ := Bundled.inst A
+  instance inst (A : univ.{u} M) : IsCategory.{max u (w + 1) iw} M ⌈A⌉ := Bundled.inst A
 
-  instance isCategory (A : univ V) : IsCategory (inst A).M := (inst A).hCategory
+  instance hasInstanceEquivalences : HasInstanceEquivalences (univ M) M.V := ⟨λ A => ⟨(inst A).Iso⟩⟩
 
-  @[reducible] def Hom {A : univ V} (a b : A) := (inst A).M a b
-  infixr:20 " ⇾ " => Category.Hom
+  class IsFun {A : univ.{u} M} {B : univ.{v} M} (φ : A → B) extends
+    IsCategoryFunctor φ : Sort (max u (w + 1) iw)
 
-  def idHom {A : univ V} (a : A) : a ⇾ a := HasRefl.refl a
-
-  -- TODO: Integrate iso into `IsCategory` and functor
-
-  class IsIso {A : univ V} {a b : A} (f : a ⇾ b) (g : b ⇾ a) where
-  (gfInv : g • f ≃ idHom a)
-  (fgInv : f • g ≃ idHom b)
-
-  namespace IsIso
-
-    instance refl {A : univ V} (a : A) : IsIso (idHom a) (idHom a) :=
-    ⟨rightId (idHom a), rightId (idHom a)⟩
-
-    instance symm {A : univ V} {a b : A}
-                  (f : a ⇾ b) (g : b ⇾ a) [isIso : IsIso f g] :
-      IsIso g f :=
-    ⟨isIso.fgInv, isIso.gfInv⟩
-
-    instance trans {A : univ V} {a b c : A}
-                   (f  : a ⇾ b) (g  : b ⇾ a) [isIso : IsIso f  g]
-                   (f' : b ⇾ c) (g' : c ⇾ b) [isIso : IsIso f' g'] :
-      IsIso (f' • f) (g • g') :=
-    ⟨sorry,
-     sorry⟩
-
-  end IsIso
-
-  structure Iso {A : univ V} (a b : A) where
-  (f     : a ⇾ b)
-  (g     : b ⇾ a)
-  [isIso : IsIso f g]
-
-  namespace Iso
-
-    instance {A : univ V} {a b : A} (e : Iso a b) : IsIso e.f e.g := e.isIso
-
-    def rel (A : univ V) : MetaRelation ⌈A⌉ sort := Iso (A := A)
-
-    instance isEquivalence (A : univ V) : IsEquivalence (rel A) :=
-    { refl  := λ a   => ⟨idHom a,   idHom a⟩,
-      symm  := λ e   => ⟨e.g,       e.f⟩,
-      trans := λ e f => ⟨f.f • e.f, e.g • f.g⟩ }
-
-    def equivalence (A : univ V) : EquivalenceRelation ⌈A⌉ sort := ⟨rel A⟩
-
-  end Iso
-
-  instance hasInstanceEquivalences : HasInstanceEquivalences (univ V) sort := ⟨Iso.equivalence⟩
-
-  class IsFun {A : univ.{u, v, iv} V} {B : univ.{u', v, iv} V} (φ : A → B) : Type (max u v iv) where
-  (mapHom             {a b : A}                           : (a ⇾ b) ⟶ (φ a ⇾ φ b))
-  (mapHom_refl        (a : A)                             : mapHom (idHom a) ≃ idHom (φ a))
-  (mapHom_trans       {a b c : A} (f : a ⇾ b) (g : b ⇾ c) : mapHom (g • f) ≃ mapHom g • mapHom f)
-  (mapHom_transExt    {a b : A} (f : a ⇾ b) (c : A)       :
-     mapHom • HasTransFun.transFun (inst A).M f c
-     ≃{byArgDef ▻ λ g => mapHom_trans f g ◅ byDef}
-     HasTransFun.transFun (inst B).M (mapHom f) (φ c) • mapHom)
-  (mapHom_transExtExt (a b c : A)                         :
-     revCompFunFun (b ⇾ c) mapHom • HasTransFun.transFunFun (inst A).M a b c
-     ≃{byDef • byArgDef ▻ λ f => mapHom_transExt f c ◅ byDef • byArgDef • byArgDef}
-     compFunFun mapHom (φ a ⇾ φ c) • HasTransFun.transFunFun (inst B).M (φ a) (φ b) (φ c) • mapHom)
-
-  instance hasFunctoriality : HasFunctoriality (typeClass.{u, v, iv} V) (typeClass.{u', v, iv} V) type.{max u v iv} :=
+  instance hasFunctoriality :
+    HasFunctoriality (typeClass.{u} M) (typeClass.{v} M) sort.{max u (w + 1) iw} :=
   ⟨IsFun⟩
 
-  instance funIsPreorder : IsPreorder (V := type.{max u v iv})
-                                      (Bundled.Fun (φ := typeClass.{u, v, iv} V) (ψ := typeClass.{u, v, iv} V)) :=
+  instance funIsCategory (A : univ.{u} M) (B : univ.{v} M) :
+    IsCategory.{max u v (w + 1) iw, w, iw} M (Bundled.Fun A B) :=
   sorry
 
-  instance funIsCategory : IsCategory (V := type.{max u v iv})
-                                      (Bundled.Fun (φ := typeClass.{u, v, iv} V) (ψ := typeClass.{u, v, iv} V)) :=
-  sorry
+  instance hasFunctorInstances :
+    HasFunctorInstances.{max u (w + 1) iw, max u (w + 1) iw, max u (w + 1) iw} (typeClass.{u} M) :=
+  ⟨funIsCategory⟩
 
-  instance hasFunctorInstances : HasFunctorInstances.{u + 1, (max u v iv) + 1, (max u v iv) + 1} (typeClass.{u, v, iv} V) :=
-  ⟨λ A B => sorry⟩
+  instance hasFunctors : HasFunctors (univ M) (univ M) (univ M) :=
+  Bundled.hasFunctors.{max u (w + 1) iw, max u (w + 1) iw, max u (w + 1) iw} (typeClass.{u} M)
 
-  instance hasFunctors : HasFunctors (univ V) (univ V) (univ V) :=
-  Bundled.hasFunctors.{u + 1, (max u v iv) + 1, (max u v iv) + 1} (typeClass.{u, v, iv} V)
-
-  instance hasCongrArg : HasCongrArg (univ V) (univ V) :=
+  instance hasCongrArg : HasCongrArg (univ M) (univ M) :=
   ⟨λ F => sorry⟩
 
-  instance hasInternalFunctors : HasInternalFunctors (univ V) := ⟨⟩
+  instance hasInternalFunctors : HasInternalFunctors (univ M) := ⟨⟩
 
-  instance hasLinearFunOp : HasLinearFunOp (univ V) := sorry
+  instance hasLinearFunOp : HasLinearFunOp (univ M) := sorry
 
-end Category
+end CategoryTheory.IsCategory
